A certifying compiler from TFL functions (in a particular form) to ARM machine code has been added. A demo of its use is in:
  arm_compiler_demoScript.sml

examples/mc-logic/arm_compilerLib.sig
@@ -1,0 +1,15 @@
+signature arm_compilerLib =
+sig
+    include Abbrev
+
+    val arm_compile         : thm -> thm -> bool -> thm * string list
+    val reset_compiled      : unit -> unit
+
+    val optimise_code       : bool ref
+    val abbrev_code         : bool ref
+
+    val show_enc            : bool ref
+    val show_code           : bool ref 
+    val pp_enc              : unit -> unit
+
+end
