examples/mc-logic/set_sepLib.sig
@@ -6,6 +6,8 @@ sig
     val dest_STAR           : term -> term * term
     val list_mk_STAR        : term list -> term
     val list_dest_STAR      : term -> term list    
+    val is_SEP_HIDE         : term -> bool
+    val get_sep_domain      : term -> term
 
     val sep_ss              : simpLib.ssfrag 
     val sep2_ss             : simpLib.ssfrag 
@@ -22,6 +24,9 @@ sig
     val MOVE_STAR_CONV      : term frag list -> term frag list -> conv
     val MOVE_STAR_RULE      : term frag list -> term frag list -> rule
 
-    val MOVE_OUT_CONV       : term frag list -> conv
+    val MOVE_OUT_TERM_CONV       : term -> conv
+    val MOVE_OUT_CONV            : term frag list -> conv
+    val MOVE_OUT_LIST_TERM_CONV  : term list -> conv
+    val MOVE_OUT_LIST_CONV       : term frag list list -> conv
 
 end
