examples/mc-logic/arm_compiler_demoScript.sml
@@ -1,0 +1,936 @@
+(*
+  fun load_path_add x = loadPath := !loadPath @ [concat Globals.HOLDIR x];
+  load_path_add "/examples/mc-logic";
+  load_path_add "/examples/ARM/v4";
+  load_path_add "/tools/mlyacc/mlyacclib";
+*)
+
+open HolKernel boolLib bossLib Parse;
+open arm_compilerLib;
+
+val _ = optimise_code := true;
+val _ = abbrev_code := false;
+
+val _ = new_theory "arm_compiler_demo";
+
+(* 
+
+INTRODUCTION
+
+This file illustrates, through examples, how the ARM compiler from 
+arm_progLib can be used. The compiler's top-level function is 
+
+  arm_progLib.arm_compile (def:thm) (ind:thm) (as_proc:bool)
+
+Here def is a definition, ind is the induction rule produced by Define
+and as_proc is a boolean flag indicating whether def should be compiled as 
+a procedure or not.
+
+In order to keep the presentation consice we define test_compile and
+test_compile_proc: 
+
+*)
+
+fun find_ind_thm def = let
+  val tm = (fst o dest_eq o concl o SPEC_ALL) def
+  val name = (fst o dest_const) ((fst o dest_comb) tm handle e => tm)
+  in fetch "-" (name^"_ind") handle e => TRUTH end;
+
+fun test_compile' as_proc q = let
+  val def = Define q
+  val ind = find_ind_thm def
+  val (th,strs) = arm_compile def ind as_proc
+ (* val _ = map print (["\n\n\n"] @ strs @ ["\n\n\n"]) *)
+  in (def,ind,th) end;
+
+fun test_compile q = test_compile' false q;
+fun test_compile_proc q = test_compile' true q;
+
+(* 
+
+The compiler expects def to be a function where variables have names 
+r0,r1,r2,...,r12 or m0,m1,m2 .... The variable names tells the compiler 
+how to assign physical resources to each logical variable, e.g.
+
+  r1  - becomes register 1
+  m5  - becomes memory location at address stack pointer + 5 
+
+The functions it accepts must conform to the following grammar.
+Let r range over register names (r0,r1,r2,etc), m range over 
+memory locations (m0,m1,m2,etc), i over natural numbers and 
+w over 8-bit word constants.
+
+  p    ::=  let r = exp in p  
+         |  let m = r in p  
+         |  if g then p else p  
+         |  (v,v,...,v)
+
+  v    ::=  r  |  m
+  g    ::=  ~ g  |  r cmp mode  |  r && mode = 0w
+  cmp  ::=  =  |  <  |  <+  |  <=  |  <=+
+  exp  ::=  m  |  mode  |  ~ mode  |  r op mode  |  r * r
+  op   ::=  + | - | && | ?? | !!
+  mode ::=  w  |  r  |  r << i  |  r >> i  |  r >>> i 
+
+Notice that one cannot have:
+
+  let r0 = (if r1 < r2 then 5w else r6) in P
+
+This needs to be expanded out as follows:
+
+  if r1 < r2 then
+    let r0 = 5w in P
+  else
+    let r0 = r6 in P
+
+A naive compilation would duplicate the code for P. We optimise
+"common code tails" and that way, to a large extent, avoid duplication 
+of code (See section of shared-tails for more).
+
+*)
+ 
+
+(* TEST: constant functions *)
+
+val (load_const_def,_,load_const_arm) = test_compile `
+  load_const : word32 # word32 # word32 =
+    let r0 = 0w in
+    let r1 = 45w in
+    let r2 = ~r1 in
+      (r0,r1,r2)`;
+
+(* Each let-expression is compiled into one ARM instruction or 
+   procedure call. The code for load_const above becomes: 
+  
+     mov r0, #0
+     mov r1, #45
+     mvn r2, r1
+*)
+
+
+(* TEST: nonrecursive functions *)
+
+val (garble_def,_,garble_arm) = test_compile `
+  garble (r2:word32,r3:word32,r4:word32) =
+    let r1 = r2 + r3 in
+    let r2 = r1 - r3 << 5 in
+    let r3 = r2 * r3 in
+    let r1 = r1 + 4w in
+    let r2 = r3 && r2 >>> 30 in
+    let r2 = r2 << 16 in
+    let r2 = ~(r2 >>> 2) in
+    let r3 = r2 !! r1 in
+    let r2 = r3 ?? 55w in
+      (r2,r3)`;
+
+(* Input and output are tuples. For garble_def we expect input in
+   register 2, 3 and 4; and produce output into registers 2 and 3. *)
+
+
+(* TEST: recursive functions *)
+
+val (mul32_def,mul32_ind,mul32_arm) = test_compile `
+  mul32 (r0:word32,r1:word32,r2:word32) =
+    if r0 = 0w then (r0,r1,r2) else 
+      let r2 = r1 + r2 in
+      let r0 = r0 - 1w in
+        mul32 (r0,r1,r2)`;
+
+val (fac32_def,fac32_ind,fac32_arm) = test_compile `
+  fac32 (r0:word32,r1:word32) =
+    if r0 = 0w then r1 else 
+      let r1 = r0 * r1 in
+      let r0 = r0 - 1w in
+        fac32 (r0,r1)`;
+
+(* Looping functions are required to be tail-recursive and
+   the recurive calls need to be identical to the left-hand side of 
+   the definition of the function, i.e. 
+     
+     f (r1,r2) = let .... in f (r2,r3)
+
+   is not allowed, since (r1,r2) is not syntactically the same as (r2,r3). *)
+
+
+(* TEST: functions with multiple recursive calls *)
+
+val (recg_def,recg_ind,recg_arm) = test_compile `
+  recg (r0:word32,r1:word32) = 
+    if r0 = 0w then 
+     r1 
+    else if r0 = 2w then 
+     (let r2 = r0 && r1 in r1) 
+    else if r0 = r1 then
+     (let r2 = 5w:word32 in
+      let r3 = ~r2 in
+      let r1 = r0 * r1 in
+      let r0 = r0 - 1w in
+        recg(r0,r1))
+    else 
+     (let r1 = r0 * r1 in
+      let r3 = ~r1 in
+      let r0 = r0 - 1w in
+        recg(r0,r1))`;
+
+
+(* TEST: negative guard in if-then-else *)
+
+val (neg_test_def,_,neg_test_arm) = test_compile `
+  neg_test (r0:word32,r1:word32) = 
+    let r1 = r0 + r1 in
+    if ~(r0 = 0w) then 
+      let r1 = r0 + r1 in
+        r1
+    else
+      let r1 = r1 + 4w in
+        r1`;
+
+
+(* TEST: various guards *)
+
+val (guard_test_def,_,guard_test_arm) = test_compile `
+  guard_test (r0:word32,r1:word32,r2:word32,r3:word32) = 
+    if 5w <= r2         then let r0 = r1 + 2w in r0 else
+    if r0 <+ 3w         then let r0 = r1 + 3w in r0 else r0`;
+
+val (guard_test_def,_,guard_test_arm) = test_compile `
+  guard_test (r0:word32,r1:word32,r2:word32,r3:word32) = 
+    if r0 <= r2         then let r0 = r1 + 2w in r0 else
+    if r0 <+ 3w         then let r0 = r1 + 3w in r0 else
+    if ~(r0 < 3w)       then let r0 = r1 + 5w in r0 else
+    if r0 <+ r3 << 2    then let r0 = r1 + 6w in r0 else
+    if r3 << 2 <+ r3    then let r0 = r1 + 7w in r0 else
+    if ~(r3 >> 2 <+ r3) then let r0 = r1 + 8w in r0 else r0`;
+
+val (guard_loop_def,guard_loop_ind,guard_loop_arm) = test_compile `
+  guard_loop (r0:word32) = 
+    if r0 = 0w then r0 else
+      if r0 < 3w then 
+        let r0 = r0 - 1w in guard_loop(r0)
+      else 
+        let r0 = r0 - 1w in guard_loop(r0)`
+
+(* Notice that one of the branches in same_guard_def is unreachable.
+   The compiler will be unable to prove the unreachable path and drops it.
+   Hence the message from the compiler                                     *)
+
+val (same_guard_def,_,same_guard_arm) = test_compile `
+  same_guard (r0:word32,r1:word32,r2:word32,r3:word32) = 
+    if r0 < 3w then let r0 = r1 + 1w in r0 else
+    if r0 < 3w then let r0 = r1 + 3w in r0 else r0`;
+
+
+(* TEST: conditional execution *)
+
+(* Here the compiler does not introduce a branch instead it executes 
+   the addition conditionally. *)
+
+val (reg_min_def,_,reg_min_arm) = test_compile `
+  reg_min (r0:word32,r1:word32) =
+    if r0 < r1 then 
+      let r1 = r1 + r0 in r1 
+    else 
+      r1`;
+
+
+(* TEST: if-then-else shared tail elim *)
+
+(* In order to avoid duplication of code the compiler can pull out
+   tails that are shared across if-then-else branches. *)
+
+val (shared_tail_def,_,shared_tail_arm) = test_compile `
+  shared_tail (r0:word32,r1:word32,r2:word32) =
+    if r1 < r2 then 
+      let r1 = r2 in
+      let r0 = r1 + 5w in
+      let r2 = r0 + r1 in
+        r2
+    else 
+      let r0 = r1 + 5w in
+      let r2 = r0 + r1 in
+        r2`;
+
+val (shared_tail2_def,_,shared_tail2_arm) = test_compile `
+  shared_tail2 (r0:word32,r1:word32,r2:word32) =
+    if r1 < r2 then
+      if r2 < r0 then 
+        let r1 = r2 + 1w in
+        let r0 = r1 - 5w in
+        let r0 = r0 - 5w in
+          r0
+      else 
+        let r1 = r2 + 2w in
+        let r0 = r1 - 5w in
+        let r0 = r0 - 5w in
+          r0
+    else 
+      if r2 < 5w then 
+        let r1 = r2 + 3w in
+        let r0 = r1 - 5w in
+        let r0 = r0 - 5w in
+          r0
+      else 
+        let r1 = r2 + 4w in
+        let r0 = r1 - 5w in
+        let r0 = r0 - 5w in
+          r0`;
+
+
+(* TEST: if-the-else shared front can be pulled out *)
+
+(* In some cases the front can be pulled out as illustrated 
+   by the following code. The comparison instruction comes first
+   in the compiled code, then the move and the addition and at 
+   the end subtraction is done conditionally. *)
+
+val (shared_front_def,_,shared_front_arm) = test_compile `
+  shared_front (r0:word32,r1:word32,r2:word32) =
+    if r1 < r2 then 
+      let r1 = 5w in
+      let r2 = r1 + r2 in
+        r2
+    else 
+      let r1 = 5w in
+      let r2 = r1 + r2 in
+      let r2 = r2 - 4w in  
+        r2`;
+
+
+(* TEST: memory accesses *)
+
+(* Memory accesses to the stack are done using variables names
+   m0,m1,m2 etc. Memory locations cannot be refered to in 
+   expressions, e.g. 
+
+     let m1 = m2 + 5w in ... 
+ 
+   is not allowed, since there is no ARM instruction for 
+   addition of memory locations. Instead:
+ 
+     let r0 = m2 in
+     let m1 = r0 + 5w in ... 
+ 
+*)
+
+val (mem_swap_def,_,mem_swap_arm) = test_compile `
+  mem_swap (m0:word32,m1:word32) =
+    let r0 = m0 in  
+    let r1 = m1 in
+    let m0 = r1 in
+    let m1 = r0 in
+      (m0,m1)`;
+
+val (mem_as_temp_def,_,mem_as_temp_arm) = test_compile `
+  mem_as_temp (r0:word32,r1:word32,r2:word32) =
+    let m1 = r0 in  
+    let r1 = r1 + r2 in
+    let m2 = r1 in
+    let r2 = r1 + r2 in
+    let m3 = r2 in
+      m3`;
+
+
+(* TEST: procedure in-lining *)
+
+(* The compiler keeps track of previously compiled code. In order to 
+   flush its memory call: 
+
+     reset_compiled() 
+*)
+
+val _ = reset_compiled();
+
+val (fac32_acc_def,fac32_acc_ind,fac32_acc_arm) = test_compile `
+  fac32_acc (r0:word32,r1:word32) =
+    if r0 = 0w then r1 else 
+      let r1 = r0 * r1 in
+      let r0 = r0 - 1w in
+        fac32_acc (r0,r1)`;
+
+val (fac32_def,_,fac32_arm) = test_compile `
+  fac32 (r0:word32) =
+    let r1 = 1w in
+    let r1 = fac32_acc (r0,r1) in
+    let r0 = r1 in
+      r0`;
+
+(* fac32 contains an instance of fac32_acc. Make sure that the
+   call to fac32_acc uses the variable names with which fac32_acc 
+   was defined, e.g. calling it using 
+
+     let r1 = fac32_acc (r3,r4) in
+     
+   is not allowed since (r3,r4) is not syntactically equal to (r0,r1)
+   which was used in the definition of fac32_acc; similarly 
+
+     let r9 = fac32_acc (r0,r1) in
+     
+   is also malformed since the result of fac32_acc is stored in r0, 
+   not in r9.
+*)
+
+(* 
+-- for some reason fac_add_def makes Holmake fail, but it's fine here.
+
+val (fac_add_def,_,fac_add_arm) = test_compile `
+  fac_add (r0:word32,r2:word32) =
+    let r0 = fac32(r0) in
+    let r0 = r0 + r2 in
+      r0`;
+*)
+
+(* Note that the compilation of fac_add would rightly fail, if r2 was 
+   replaced by r1 in the definition of fac_add, since r1 is used 
+   when fac32 executes. *)
+
+
+
+(* TEST: procedure calls *)
+
+val _ = reset_compiled();
+
+(* If we compile fac32_acc as a procedure then calls to it will be 
+   executed using the ARM instruction for procedure calls, i.e.
+   the BL instruction (branch-and-link). *)
+
+val (fac32_acc_def,fac32_acc_ind,fac32_acc_arm) = test_compile_proc `
+  fac32_acc (r0:word32,r1:word32) =
+    if r0 = 0w then r1 else 
+      let r1 = r0 * r1 in
+      let r0 = r0 - 1w in
+        fac32_acc (r0,r1)`;
+
+val (fac32_def,_,fac32_arm) = test_compile `
+  fac32 (r0:word32) =
+    let r1 = 1w in
+    let r1 = fac32_acc (r0:word32,r1:word32) in
+    let r0 = r1 in
+      r0`;
+
+(* Note: At present, it is only possible to do subroutine calls to a 
+   depth of one, since the link-register (register 14) gets garbled 
+   if a subroutine call is made inside a subroutine. Arbitrary 
+   depth procedure calls will soon be implemented. *)
+
+
+(* TEST: Joe's ECC definitions *)
+
+(* The code becomes very large (thousands of lines) in the following 
+   examples since we use procedure in-lineing through out.
+   Hence, in order to cope we switch on "code abbrevaition". *)
+
+val _ = abbrev_code := true;
+
+
+val _ = reset_compiled();
+
+val (load_751_def,_,load_751_arm) = test_compile `
+  load_751 = 
+    let r10 = 2w:word32 in
+    let r10 = r10 << 8 in
+    let r10 = r10 + 239w in r10`;
+
+val (field_neg_def,_,field_neg_arm) = test_compile `
+  field_neg (r1:word32) =
+    if r1 = 0w then r1 else 
+      let r10 = load_751 in
+      let r1 = r10 - r1 in r1`;
+
+val (field_add_def,_,field_add_arm) = test_compile `
+  field_add (r0:word32,r1:word32) =
+    let r10 = load_751 in
+    let r0 = r1 + r0 in
+      if r0 < r10 then r0 else 
+        let r0 = r0 - r10 in 
+          r0`;
+
+val (field_sub_def,_,field_sub_arm) = test_compile `
+  field_sub (r0,r1) =
+    let r1 = field_neg r1 in 
+    let r0 = field_add (r0,r1) in 
+      r0`;
+
+val (field_mult_aux_def,field_mult_aux_ind,field_mult_aux_arm) = test_compile `
+  field_mult_aux (r2:word32,r3:word32,r4:word32) =
+    if r3 = 0w then r4 else
+      if r3 && 1w = 0w then 
+          let r3 = r3 >>> 1 in 
+          let r0 = r2 in
+          let r1 = r2 in
+          let r0 = field_add (r0,r1) in
+          let r2 = r0 in
+            field_mult_aux (r2:word32,r3:word32,r4:word32)
+        else
+          let r3 = r3 >>> 1 in 
+          let r0 = r4 in
+          let r1 = r2 in
+          let r0 = field_add (r0,r1) in
+          let r4 = r0 in
+          let r0 = r2 in
+          let r1 = r2 in
+          let r0 = field_add (r0,r1) in
+          let r2 = r0 in
+            field_mult_aux (r2:word32,r3:word32,r4:word32)`;
+
+val (field_mult_def,_,field_mult_arm) = test_compile `
+  field_mult (r2,r3) = 
+    let r4 = 0w in
+    let r4 = field_mult_aux (r2,r3,r4) in
+      r4`;
+
+val (field_exp_aux_def,field_exp_aux_ind,field_exp_aux_arm) = test_compile `
+  field_exp_aux (r5:word32,r6:word32,r7:word32) =
+    if r6 = 0w then r7 else
+      if r6 && 1w = 0w then 
+          let r6 = r6 >>> 1 in 
+          let r2 = r5 in
+          let r3 = r5 in
+          let r4 = field_mult (r2,r3) in
+          let r5 = r4 in
+            field_exp_aux (r5:word32,r6:word32,r7:word32)
+        else
+          let r6 = r6 >>> 1 in 
+          let r2 = r7 in
+          let r3 = r5 in
+          let r4 = field_mult (r2,r3) in
+          let r7 = r4 in
+          let r2 = r5 in
+          let r3 = r5 in
+          let r4 = field_mult (r2,r3) in
+          let r5 = r4 in
+            field_exp_aux (r5:word32,r6:word32,r7:word32)`;
+
+val (field_exp_def,_,field_exp_arm) = test_compile `
+  field_exp (r5,r6) = 
+    let r7 = 1w in
+    let r7 = field_exp_aux (r5,r6,r7) in
+      r7`;
+
+val (field_inv_def,_,field_inv_arm) = test_compile `
+  field_inv r5 = 
+    let r6 = 2w:word32 in
+    let r6 = r6 << 8 in
+    let r6 = r6 + 237w in 
+    let r7 = field_exp (r5,r6) in
+      r7`;
+
+val (field_div_def,_,field_div_arm) = test_compile `
+  field_div (r8,r9) = 
+    let r5 = r9 in
+    let r7 = field_inv r5 in
+    let r2 = r8 in
+    let r3 = r7 in
+    let r4 = field_mult(r2,r3) in
+      r4`;
+  
+val (both_zero_def,_,both_zero_arm) = test_compile `
+  both_zero (r1:word32,r2:word32) =
+    if r1 = 0w then 
+      if r2 = 0w then 
+        let r0 = 1w:word32 in (r0,r1,r2)
+      else 
+        let r0 = 0w in (r0,r1,r2)
+    else
+      let r0 = 0w in (r0,r1,r2)`;
+
+val (both_eq_def,_,both_eq_arm) = test_compile `
+  both_eq (r1:word32,r2:word32,r3:word32,r4:word32) =
+    if r1 = r3 then 
+      if r2 = r4 then 
+        let r0 = 1w:word32 in (r0,r1,r2,r3,r4)
+      else 
+        let r0 = 0w in (r0,r1,r2,r3,r4)
+    else
+      let r0 = 0w in (r0,r1,r2,r3,r4)`;
+
+val (curve_neg_def,_,curve_neg_arm) = test_compile `
+  curve_neg (r1:word32,r2:word32) =
+    let (r0,r1,r2) = both_zero(r1,r2) in
+      if r0 = 0w then 
+        (r1,r2) 
+      else
+        let r8 = r1 in
+        let r9 = r2 in
+        let r2 = 0w in
+        let r3 = r8 in
+        let r4 = field_mult(r2,r3) in
+        let r1 = r9 in
+        let r1 = field_neg r1 in
+        let r0 = r1 in
+        let r1 = r4 in
+        let r0 = field_sub(r0,r1) in
+        let r1 = 1w in
+        let r0 = field_sub(r0,r1) in
+        let r2 = r0 in
+        let r1 = r8 in
+          (r1,r2)`;
+
+val (curve_double_def,_,curve_double_arm) = test_compile `
+  curve_double (r1,r2) =
+    let (r0,r1,r2) = both_zero(r1,r2) in
+    if r0 = 0w then (r1,r2) else
+    let m1 = r1 in (* x1 *)
+    let m2 = r2 in (* y1 *)
+    let r2 = 2w in
+    let r3 = r2 in
+    let r4 = field_mult(r2,r3) in
+    let r5 = r4 in
+    let r2 = 0w in
+    let r3 = m1 in
+    let r4 = field_mult(r2,r3) in
+    let r0 = r5 in      
+    let r1 = r4 in      
+    let r0 = field_add(r0,r1) in
+    let r1 = 1w in      
+    let r0 = field_add(r0,r1) in
+    if r0 = 0w then 
+      let r1 = 1w in
+      let r2 = 0w in
+        (r1,r2)
+    else
+    let r11 = r0 in (* d *)
+    let r5 = m1 in
+    let r6 = 2w in
+    let r7 = field_exp(r5,r6) in
+    let r2 = 3w in
+    let r3 = r7 in    
+    let r4 = field_mult(r2,r3) in
+    let r8 = r4 in
+    let r2 = 2w in
+    let r3 = 0w in    
+    let r4 = field_mult(r2,r3) in
+    let r3 = m1 in
+    let r2 = r4 in
+    let r4 = field_mult(r2,r3) in
+    let r0 = r8 in
+    let r1 = r4 in
+    let r0 = field_add(r0,r1) in
+    let r10 = load_751 in
+    let r1 = r10 - 1w in
+    let r0 = field_add(r0,r1) in
+    let r9 = r0 in
+    let r3 = m2 in
+    let r2 = 0w in
+    let r4 = field_mult(r2,r3) in
+    let r0 = r9 in
+    let r1 = r4 in
+    let r0 = field_sub(r0,r1) in
+    let r8 = r0 in    
+    let r9 = r11 in    
+    let r4 = field_div(r8,r9) in
+    let r12 = r4 in (* l *)
+    let r5 = m1 in
+    let r6 = 3w in
+    let r7 = field_exp(r5,r6) in
+    let r1 = r7 in
+    let r1 = field_neg r1 in
+    let r7 = r1 in
+    let r10 = load_751 in
+    let r3 = m1 in
+    let r2 = r10 - 1w in    
+    let r4 = field_mult(r2,r3) in
+    let r0 = r7 in
+    let r1 = r4 in
+    let r0 = field_add(r0,r1) in
+    let r7 = r0 in
+    let r2 = 2w in
+    let r3 = 0w in
+    let r4 = field_mult(r2,r3) in
+    let r0 = r7 in
+    let r1 = r4 in
+    let r0 = field_add(r0,r1) in
+    let r9 = r0 in
+    let r3 = m2 in
+    let r2 = 1w in    
+    let r4 = field_mult(r2,r3) in
+    let r0 = r9 in
+    let r1 = r4 in
+    let r0 = field_sub(r0,r1) in
+    let r8 = r0 in
+    let r9 = r11 in
+    let r4 = field_div(r8,r9) in
+    let r11 = r4 in (* m *)
+    let r5 = r12 in
+    let r6 = 2w in    
+    let r7 = field_exp(r5,r6) in
+    let r2 = 0w in
+    let r3 = r12 in    
+    let r4 = field_mult(r2,r3) in
+    let r0 = r7 in 
+    let r1 = r4 in 
+    let r0 = field_add(r0,r1) in
+    let r1 = 0w in 
+    let r0 = field_sub(r0,r1) in
+    let r7 = r0 in
+    let r3 = m1 in    
+    let r2 = 2w in
+    let r4 = field_mult(r2,r3) in
+    let r0 = r7 in
+    let r1 = r4 in
+    let r0 = field_sub(r0,r1) in
+    let r9 = r0 in (* x *)
+    let r0 = r12 in 
+    let r1 = 0w in 
+    let r0 = field_add(r0,r1) in
+    let r1 = r0 in
+    let r1 = field_neg r1 in
+    let r2 = r1 in    
+    let r3 = r9 in    
+    let r4 = field_mult(r2,r3) in
+    let r0 = r4 in
+    let r1 = r11 in 
+    let r0 = field_sub(r0,r1) in
+    let r1 = 1w in 
+    let r0 = field_sub(r0,r1) in
+    let r2 = r0 in (* y *)
+    let r1 = r9 in (* x *)
+      (r1,r2)`;
+
+val (curve_add_def,_,curve_add_arm) = test_compile `
+  curve_add (r1,r2,r3,r4) =
+    let (r0,r1,r2,r3,r4) = both_eq(r1,r2,r3,r4) in
+    if r0 = 0w then 
+      let (r1,r2) = curve_double (r1,r2) in
+        (r1,r2)
+    else      
+    let (r0,r1,r2) = both_zero(r1,r2) in
+    if r0 = 0w then 
+      let r1 = r3 in
+      let r2 = r4 in
+        (r1,r2) 
+    else 
+    let m1 = r1 in (* x1 *)
+    let m2 = r2 in (* y1 *)
+    let m3 = r3 in (* x2 *)
+    let m4 = r4 in (* y2 *)
+    let r1 = r3 in
+    let r2 = r4 in
+    let (r0,r1,r2) = both_zero(r1,r2) in
+    if r0 = 0w then 
+      let r1 = m1 in
+      let r2 = m2 in
+        (r1,r2) 
+    else        
+    let r0 = m1 in
+    if r0 = r1 then
+      let r1 = 0w in
+      let r2 = 0w in
+        (r1,r2)
+    else
+    let r0 = m3 in
+    let r1 = m1 in
+    let r0 = field_sub(r0,r1) in
+    let r11 = r0 in (* d *)
+    let r0 = m4 in
+    let r1 = m2 in
+    let r0 = field_sub(r0,r1) in
+    let r8 = r0 in
+    let r9 = r11 in
+    let r4 = field_div(r8,r9) in
+    let r12 = r4 in (* l *)      
+    let r2 = m2 in    
+    let r3 = m3 in    
+    let r4 = field_mult(r2,r3) in
+    let r9 = r4 in
+    let r2 = m4 in    
+    let r3 = m1 in    
+    let r4 = field_mult(r2,r3) in
+    let r0 = r9 in
+    let r1 = r4 in
+    let r0 = field_sub(r0,r1) in
+    let r8 = r0 in
+    let r9 = r11 in
+    let r4 = field_div(r8,r9) in
+    let r11 = r4 in (* m *)
+    let r2 = 0w in
+    let r3 = r12 in 
+    let r4 = field_mult(r2,r3) in
+    let r9 = r4 in
+    let r5 = r12 in
+    let r6 = 2w in
+    let r7 = field_exp(r5,r6) in
+    let r0 = r7 in
+    let r1 = r9 in
+    let r0 = field_add(r0,r1) in
+    let r1 = 0w in
+    let r0 = field_sub(r0,r1) in
+    let r1 = m1 in
+    let r0 = field_sub(r0,r1) in
+    let r1 = m3 in
+    let r0 = field_sub(r0,r1) in
+    let r9 = r0 in (* x *)
+    let r0 = r12 in
+    let r1 = 0w in
+    let r0 = field_add(r0,r1) in
+    let r1 = r0 in
+    let r1 = field_neg r1 in
+    let r2 = r1 in
+    let r3 = r9 in
+    let r4 = field_mult(r2,r3) in
+    let r0 = r4 in
+    let r1 = r11 in
+    let r0 = field_sub(r0,r1) in
+    let r1 = 1w in
+    let r0 = field_sub(r0,r1) in (* y *)
+    let r1 = r9 in
+    let r2 = r0 in
+      (r1,r2)`;
+
+val (curve_mult_aux_def,curve_mult_aux_ind,curve_mult_aux_arm) = test_compile `
+  curve_mult_aux (m5:word32,m6:word32,m7:word32,m8:word32,m9:word32) =
+    let r0 = m7 in
+    if r0 = 0w then (m8,m9) else
+      if r0 && 1w = 0w then 
+          let r0 = r0 >>> 1 in 
+          let r1 = m5 in
+          let r2 = m6 in
+          let m7 = r0 in
+          let (r1,r2) = curve_double (r1,r2) in
+          let m5 = r1 in
+          let m6 = r2 in
+            curve_mult_aux (m5,m6,m7,m8,m9)
+        else
+          let r0 = r0 >>> 1 in 
+          let r1 = m5 in
+          let r2 = m6 in
+          let r3 = m8 in
+          let r4 = m9 in
+          let m7 = r0 in
+          let (r1,r2) = curve_add (r1,r2,r3,r4) in
+          let m8 = r1 in
+          let m9 = r2 in
+          let r1 = m5 in
+          let r2 = m6 in
+          let (r1,r2) = curve_double (r1,r2) in
+          let m5 = r1 in
+          let m6 = r2 in
+            curve_mult_aux (m5,m6,m7,m8,m9)`;
+
+val (curve_mult_def,_,curve_mult_arm) = test_compile `
+  curve_mult (r1:word32,r2:word32,r3:word32) =
+    let r0 = 0w in
+    let m5 = r1 in
+    let m6 = r2 in
+    let m7 = r3 in
+    let m8 = r0 in
+    let m9 = r0 in
+    let (m8,m9) = curve_mult_aux (m5,m6,m7,m8,m9) in
+    let r1 = m8 in
+    let r2 = m9 in
+      (r1,r2)`
+
+(*
+
+
+
+
+
+
+
+
+(* ----------------- *)
+
+val _ = reset_compiled();
+val _ = abbrev_code := true;
+
+val (load_751_def,_,load_751_arm) = test_compile `
+  load_751 = 
+    let r10 = 2w:word32 in
+    let r10 = r10 << 8 in
+    let r10 = r10 + 239w in r10`;
+
+val (field_neg_def,_,field_neg_arm) = test_compile `
+  field_neg (r1:word32,r10:word32) =
+    if r1 = 0w then (r1,r10) else 
+      let r1 = r10 - r1 in (r1,r10)`;
+
+val (field_add_def,_,field_add_arm) = test_compile `
+  field_add (r0:word32,r1:word32,r10:word32) =
+    let r0 = r1 + r0 in
+      if r0 < r10 then (r0,r10) else 
+        let r0 = r0 - r10 in 
+          (r0,r10)`;
+
+val (field_sub_def,_,field_sub_arm) = test_compile `
+  field_sub (r0:word32,r1:word32,r10:word32) =
+    let (r1,r10) = field_neg (r1,r10) in 
+    let (r0,r10) = field_add (r0,r1,r10) in 
+      (r0,r10)`;
+
+val (field_mult_aux_def,field_mult_aux_ind,field_mult_aux_arm) = test_compile `
+  field_mult_aux5 (r2:word32,r3:word32,r4:word32,r10:word32) =
+    if r3 = 0w then (r4,r10) else
+      if r3 && 1w = 0w then 
+          let r3 = r3 >>> 1 in 
+          let r0 = r2 in
+          let r1 = r2 in
+          let (r0,r10) = field_add (r0,r1,r10) in
+          let r2 = r0 in
+            field_mult_aux5 (r2,r3,r4,r10)
+        else
+          let r3 = r3 >>> 1 in 
+          let r0 = r4 in
+          let r1 = r2 in
+          let (r0,r10) = field_add (r0,r1,r10) in
+          let r4 = r0 in
+          let r0 = r2 in
+          let r1 = r2 in
+          let (r0,r10) = field_add (r0,r1,r10) in
+          let r2 = r0 in
+            field_mult_aux5 (r2,r3,r4,r10)`;
+
+val (field_mult_def,_,field_mult_arm) = test_compile `
+  field_mult (r2,r3,r10) = 
+    let r4 = 0w in
+    let (r4,r10) = field_mult_aux5 (r2,r3,r4,r10) in
+      (r4,r10)`;
+
+val (field_exp_aux_def,field_exp_aux_ind,field_exp_aux_arm) = test_compile `
+  field_exp_aux (r5:word32,r6:word32,r7:word32,r10) =
+    if r6 = 0w then (r7,r10) else
+      if r6 && 1w = 0w then 
+          let r6 = r6 >>> 1 in 
+          let r2 = r5 in
+          let r3 = r5 in
+          let (r4,r10) = field_mult (r2,r3,r10) in
+          let r5 = r4 in
+            field_exp_aux (r5,r6,r7,r10)
+        else
+          let r6 = r6 >>> 1 in 
+          let r2 = r7 in
+          let r3 = r5 in
+          let (r4,r10) = field_mult (r2,r3,r10) in
+          let r7 = r4 in
+          let r2 = r5 in
+          let r3 = r5 in
+          let (r4,r10) = field_mult (r2,r3,r10) in
+          let r5 = r4 in
+            field_exp_aux (r5,r6,r7,r10)`;
+
+val (field_exp_def,_,field_exp_arm) = test_compile `
+  field_exp (r5,r6,r10) = 
+    let r7 = 1w in
+    let (r7,r10) = field_exp_aux (r5,r6,r7,r10) in
+      (r7,r10)`;
+
+val (field_inv_def,_,field_inv_arm) = test_compile `
+  field_inv (r5,r10) = 
+    let r6 = 2w:word32 in
+    let r6 = r6 << 8 in
+    let r6 = r6 + 237w in 
+    let (r7,r10) = field_exp (r5,r6,r10) in
+      (r7,r10)`;
+
+val (field_div_def,_,field_div_arm) = test_compile `
+  field_div (r8,r9,r10) = 
+    let r5 = r9 in
+    let (r7,r10) = field_inv (r5,r10) in
+    let r2 = r8 in
+    let r3 = r7 in
+    let (r4,r10) = field_mult(r2,r3,r10) in
+      (r4,r10)`;
+
+*)
+
+val _ = export_theory();
+
